Merge reg from Andrew: split general purpose and special purpose registers.

src/amd64/reg.v
@@ -10,37 +10,45 @@ From Ssreflect Require Import eqtype ssrnat seq choice.
 From Ssreflect Require Import fintype tuple.
 Require Import bitsrep.
 
-(* TODO: check that RSP can be used as an index register on x86-64 with  *)
-(* REX.X = 1 and index = 0100 in SIB, although GNU AS doesn't seem to *)
-(* accept it. *)
+Inductive nonSPReg := 
+  RAX | RBX | RCX | RDX | RSI | RDI | RBP
+| R8  | R9  | R10 | R11 | R12 | R13 | R14 | R15.
+
+Definition encode_nonSPReg r :=
+  match r with
+    | RAX => 0 | RCX => 1 | RDX => 2 | RBX => 3 | RBP => 5 | RSI => 6 | RDI => 7 
+    | R8 => 8 | R9 => 9 | R10 => 10 | R11 => 11 | R12 => 12
+    | R13 => 13 | R14 => 14 | R15 => 15
+  end.
+Lemma encode_nonSPReg_inj : injective encode_nonSPReg. Proof. by repeat case => //. Qed.
+Canonical Structure nonSPRegEqMixin := InjEqMixin encode_nonSPReg_inj.
+Canonical Structure nonSPReg_EqType := Eval hnf in EqType _ nonSPRegEqMixin.
 
 (* General Purpose Registers *)
-Inductive gpReg := RAX | RBX | RCX | RDX | RSI | RDI | RBP | RSP | R8 | R9
-               | R10 | R11 | R12 | R13 | R14 | R15.
+
+Inductive gpReg := mkGPReg (r: nonSPReg) :> gpReg | RSP.
 
 Definition encode_gpReg r :=
   match r with
-  | RAX => 0  | RBX => 3  | RCX => 1  | RDX => 2  | RSI => 6  | RDI => 7
-  | RSP => 4  | RBP => 5  | R8 => 8   | R9 => 9  | R10 => 10 | R11 => 11
-  | R12 => 12 | R13 => 13 | R14 => 14 | R15 => 15
+    | RSP => 4
+    | mkGPReg r => encode_nonSPReg r
   end.
-
-Lemma encode_gpReg_inj : injective encode_gpReg.
-Proof. by case => //; case => //. Qed.
-
+Lemma encode_gpReg_inj : injective encode_gpReg. Proof. by repeat case => //. Qed.
 Canonical Structure gpRegEqMixin := InjEqMixin encode_gpReg_inj.
 Canonical Structure gpReg_eqType := Eval hnf in EqType _ gpRegEqMixin.
 
-Definition decode_gpReg n :=
+Definition decode_gpReg n: option gpReg :=
   match n with
-  | 0 => Some RAX  | 1 => Some RCX  | 2 => Some RDX  | 3 => Some RBX
-  | 4 => Some RSP  | 5 => Some RBP  | 6 => Some RSI  | 7 => Some RDI
-  | 8 => Some R8   | 9 => Some R9   | 10 => Some R10 | 11 => Some R11
-  | 12 => Some R12 | 13 => Some R13 | 14 => Some R14 | _ => None
+    | 0 => Some (RAX:gpReg)  | 1 => Some (RCX:gpReg)  | 2 => Some (RDX:gpReg)
+    | 3 => Some (RBX:gpReg) | 4 => Some (RSP:gpReg)   | 5 => Some (RBP:gpReg)
+    | 6 => Some (RSI:gpReg)  | 7 => Some (RDI:gpReg)  | 8 => Some (R8:gpReg)
+    | 9 => Some (R9:gpReg)   | 10 => Some (R10:gpReg) | 11 => Some (R11:gpReg)
+    | 12 => Some (R12:gpReg) | 13 => Some (R13:gpReg) | 14 => Some (R14:gpReg)
+    | _ => None
   end.
 
 (* All registers, including RIP but excluding RFL *)
-Inductive reg := GPReg (r : gpReg) | RIP.
+Inductive reg := GPReg (r: gpReg) | RIP.
 
 Coercion GPReg : gpReg >-> reg.
 
@@ -57,6 +65,7 @@ Canonical Structure regEqMixin := InjEqMixin encode_reg_inj.
 Canonical Structure reg_eqType := Eval hnf in EqType _ regEqMixin.
 
 (* Segment registers *)
+
 Inductive segReg := CS | FS | GS.
 
 Definition encode_segReg r :=
@@ -67,87 +76,197 @@ Proof. by case; case. Qed.
 Canonical Structure segRegEqMixin := InjEqMixin encode_segReg_inj.
 Canonical Structure segReg_eqType := Eval hnf in EqType _ segRegEqMixin.
 
+
 (* Low byte registers, wrapping underlying 64-bit registers *)
-Inductive BYTELReg := mkByteLReg (r : gpReg).
-Notation AL := (mkByteLReg RAX).
-Notation BL := (mkByteLReg RBX).
-Notation CL := (mkByteLReg RCX).
-Notation DL := (mkByteLReg RDX).
-Notation SIL := (mkByteLReg RSI).
-Notation DIL := (mkByteLReg RDI).
-Notation BPL := (mkByteLReg RBP).
-Notation SPL := (mkByteLReg RSP).
-Notation R8B := (mkByteLReg R8).
-Notation R9B := (mkByteLReg R9).
-Notation R10B := (mkByteLReg R10).
-Notation R11B := (mkByteLReg R11).
-Notation R12B := (mkByteLReg R12).
-Notation R13B := (mkByteLReg R13).
-Notation R14B := (mkByteLReg R14).
-Notation R15B := (mkByteLReg R15).
+Inductive nonSPReg8 := mkNonSPReg8 (r: nonSPReg).
+Inductive gpReg8 := mkGPReg8 (r: gpReg)  (*| AH | BH | CH | DH *).
+Definition BYTELReg := gpReg8.
+
+Definition NonSPReg8_base r8 := let: mkNonSPReg8 r := r8 in r.
+Coercion NonSPReg8_to_gpReg8 (r: nonSPReg8): gpReg8 := mkGPReg8 (NonSPReg8_base r).
+
+Lemma NonSPReg8_base_inj : injective NonSPReg8_base.
+Proof. move => [x] [y] [/=E]. by subst. Qed.
+Canonical Structure NonSPReg8_EqMixin := InjEqMixin NonSPReg8_base_inj.
+Canonical Structure NonSPReg8_EqType := Eval hnf in EqType _ NonSPReg8_EqMixin.
+
+Definition encode_gpReg8 r8 := 
+  match r8 with mkGPReg8 r => encode_gpReg r end.
+Lemma encode_gpReg8_inj : injective encode_gpReg8.
+Proof. repeat case => //; case => //.  Qed. 
+Canonical Structure GPReg8_EqMixin := InjEqMixin encode_gpReg8_inj.
+Canonical Structure GPReg8_EqType := Eval hnf in EqType _ GPReg8_EqMixin.
+
+
+Definition AL := (mkNonSPReg8 RAX).
+Definition BL := (mkNonSPReg8 RBX).
+Definition CL := (mkNonSPReg8 RCX).
+Definition DL := (mkNonSPReg8 RDX).
+Definition SIL := (mkNonSPReg8 RSI).
+Definition DIL := (mkNonSPReg8 RDI).
+Definition BPL := (mkNonSPReg8 RBP).
+Definition R8L := (mkNonSPReg8 R8).
+Definition R9L := (mkNonSPReg8 R9).
+Definition R10L := (mkNonSPReg8 R10).
+Definition R11L := (mkNonSPReg8 R11).
+Definition R12L := (mkNonSPReg8 R12).
+Definition R13L := (mkNonSPReg8 R13).
+Definition R14L := (mkNonSPReg8 R14).
+Definition R15L := (mkNonSPReg8 R15).
+Definition SPL := (mkGPReg8 RSP).
 
 (* High byte registers are not addressable with REX prefix *)
 Inductive BYTEHReg := AH|BH|CH|DH.
 
 (* 16-bit registers, wrapping underlying 64-bit registers *)
-Inductive WORDReg := mkWordReg (r : gpReg).
-Notation AX := (mkWordReg RAX).
-Notation BX := (mkWordReg RBX).
-Notation CX := (mkWordReg RCX).
-Notation DX := (mkWordReg RDX).
-Notation SI := (mkWordReg RSI).
-Notation DI := (mkWordReg RDI).
-Notation BP := (mkWordReg RBP).
-Notation SP := (mkWordReg RSP).
-Notation R8W := (mkWordReg R8).
-Notation R9W := (mkWordReg R9).
-Notation R10W := (mkWordReg R10).
-Notation R11W := (mkWordReg R11).
-Notation R12W := (mkWordReg R12).
-Notation R13W := (mkWordReg R13).
-Notation R14W := (mkWordReg R14).
-Notation R15W := (mkWordReg R15).
+Inductive nonSPReg16 := mkNonSPReg16 (r: nonSPReg).
+Inductive gpReg16 := mkGPReg16 (r: gpReg).
+Inductive WORDReg := mkReg16 (r: reg).
+
+Definition nonSPReg16_base r16 := let: mkNonSPReg16 r := r16 in r.
+Coercion NonSPReg16_to_GPReg16 (r: nonSPReg16) := mkGPReg16 (nonSPReg16_base r).
+
+Definition GPReg16_base r16 := let: mkGPReg16 r := r16 in r.
+Coercion GPReg16_to_Reg16 (r: gpReg16) := mkReg16 (GPReg16_base r).
+
+Definition Reg16_base r16 := let: mkReg16 r := r16 in r.
+
+Lemma nonSPReg16_base_inj : injective nonSPReg16_base.
+Proof. move => [x] [y] [/=E]. by subst. Qed. 
+Canonical Structure nonSPReg16_EqMixin := InjEqMixin nonSPReg16_base_inj.
+Canonical Structure nonSPReg16_EqType := Eval hnf in EqType _ nonSPReg16_EqMixin.
+
+Lemma GPReg16_base_inj : injective GPReg16_base.
+Proof. move => [x] [y] [/=E]. by subst. Qed. 
+Canonical Structure GPReg16_EqMixin := InjEqMixin GPReg16_base_inj.
+Canonical Structure GPReg16_EqType := Eval hnf in EqType _ GPReg16_EqMixin.
+
+Lemma Reg16_base_inj : injective Reg16_base. Proof. move => [x] [y] [/=E]. by subst. Qed. 
+Canonical Structure Reg16_EqMixin := InjEqMixin Reg16_base_inj.
+Canonical Structure Reg16_EqType := Eval hnf in EqType _ Reg16_EqMixin.
+
+
+Definition AX := (mkNonSPReg16 RAX).
+Definition BX := (mkNonSPReg16 RBX).
+Definition CX := (mkNonSPReg16 RCX).
+Definition DX := (mkNonSPReg16 RDX).
+Definition SI := (mkNonSPReg16 RSI).
+Definition DI := (mkNonSPReg16 RDI).
+Definition BP := (mkNonSPReg16 RBP).
+Definition R8W := (mkNonSPReg16 R8).
+Definition R9W := (mkNonSPReg16 R9).
+Definition R10W := (mkNonSPReg16 R10).
+Definition R11W := (mkNonSPReg16 R11).
+Definition R12W := (mkNonSPReg16 R12).
+Definition R13W := (mkNonSPReg16 R13).
+Definition R14W := (mkNonSPReg16 R14).
+Definition R15W := (mkNonSPReg16 R15).
+Definition SP := (mkGPReg16 RSP).
+Definition IP := (mkReg16 RIP).
 
 (* 32-bit registers, wrapping underlying 64-bit registers *)
-Inductive DWORDReg := mkDWordReg (r : gpReg).
-Notation EAX := (mkDWordReg RAX).
-Notation EBX := (mkDWordReg RBX).
-Notation ECX := (mkDWordReg RCX).
-Notation EDX := (mkDWordReg RDX).
-Notation ESI := (mkDWordReg RSI).
-Notation EDI := (mkDWordReg RDI).
-Notation EBP := (mkDWordReg RBP).
-Notation ESP := (mkDWordReg RSP).
-Notation R8D := (mkDWordReg R8).
-Notation R9D := (mkDWordReg R9).
-Notation R10D := (mkDWordReg R10).
-Notation R11D := (mkDWordReg R11).
-Notation R12D := (mkDWordReg R12).
-Notation R13D := (mkDWordReg R13).
-Notation R14D := (mkDWordReg R14).
-Notation R15D := (mkDWordReg R15).
+Inductive nonSPReg32 := mkNonSPReg32 (r: nonSPReg).
+Inductive gpReg32 := mkGPReg32 (r: gpReg).
+Inductive DWORDReg := mkReg32 (r: reg).
 
-Definition gpVReg (s: opsize) :=
+Definition nonSPReg32_base r32 := let: mkNonSPReg32 r := r32 in r.
+Coercion NonSPReg32_to_GPReg32 (r: nonSPReg32): gpReg32 := mkGPReg32 (nonSPReg32_base r).
+Definition gpReg32_base r32 := let: mkGPReg32 r := r32 in r.
+Coercion gpReg32_to_Reg32 (r: gpReg32): DWORDReg := mkReg32 (gpReg32_base r).
+
+Lemma NonSPReg32_base_inj : injective nonSPReg32_base.
+Proof. move => [x] [y] [/=E]. by subst. Qed. 
+Canonical Structure NonSPReg32_EqMixin := InjEqMixin NonSPReg32_base_inj.
+Canonical Structure NonSPReg32_EqType := Eval hnf in EqType _ NonSPReg32_EqMixin.
+
+Lemma GPReg32_base_inj : injective gpReg32_base. Proof. move => [x] [y] [/=E]. by subst. Qed.
+Canonical Structure GPReg32_EqMixin := InjEqMixin GPReg32_base_inj.
+Canonical Structure GPReg32_EqType := Eval hnf in EqType _ GPReg32_EqMixin.
+
+
+Definition EAX := (mkNonSPReg32 RAX).
+Definition EBX := (mkNonSPReg32 RBX).
+Definition ECX := (mkNonSPReg32 RCX).
+Definition EDX := (mkNonSPReg32 RDX).
+Definition ESI := (mkNonSPReg32 RSI).
+Definition EDI := (mkNonSPReg32 RDI).
+Definition EBP := (mkNonSPReg32 RBP).
+Definition R8D := (mkNonSPReg32 R8).
+Definition R9D := (mkNonSPReg32 R9).
+Definition R10D := (mkNonSPReg32 R10).
+Definition R11D := (mkNonSPReg32 R11).
+Definition R12D := (mkNonSPReg32 R12).
+Definition R13D := (mkNonSPReg32 R13).
+Definition R14D := (mkNonSPReg32 R14).
+Definition R15D := (mkNonSPReg32 R15).
+Definition ESP := (mkGPReg32 RSP).
+Definition EIP := (mkReg32 RIP).
+
+
+Definition nonSPVReg (s: opsize) := 
   match s with
-  | OpSize1 => BYTELReg
-  | OpSize2 => WORDReg
-  | OpSize4 => DWORDReg
-  | OpSize8 => gpReg
+    | OpSize1 => nonSPReg8
+    | OpSize2 => nonSPReg16
+    | OpSize4 => nonSPReg32
+    | OpSize8 => nonSPReg
+  end.
+
+Definition gpVReg (s: opsize) := 
+  match s with
+    | OpSize1 => gpReg8
+    | OpSize2 => gpReg16
+    | OpSize4 => gpReg32
+    | OpSize8 => gpReg
   end.
 
 Definition vreg (s: opsize) :=
   match s with
-  | OpSize1 => BYTELReg
-  | OpSize2 => WORDReg
-  | OpSize4 => DWORDReg
-  | OpSize8 => reg
+    | OpSize1 => BYTELReg
+    | OpSize2 => WORDReg
+    | OpSize4 => DWORDReg
+    | OpSize8 => reg
   end.
 
+(*
 Coercion RegToVReg (r: gpReg) : gpVReg OpSize8 := r.
-Coercion DWORDRegToVReg (r:DWORDReg) : gpVReg OpSize4 := r.
-Coercion WORDRegToVReg (r:WORDReg) : gpVReg OpSize2 := r.
-Coercion BYTELRegToVReg (r:BYTELReg) : gpVReg OpSize1 := r.
+Coercion DWORDRegToVReg (r:DWORDReg) : vreg OpSize4 := r.
+Coercion WORDRegToVReg (r:WORDReg) : vreg OpSize2 := r.
+Coercion BYTELRegToVReg (r:BYTELReg) : vreg OpSize1 := r.
 Coercion AnyRegToVRegAny (r: reg) : vreg OpSize8 := r.
+ *)
+
+Coercion nonSPVReg_to_vreg {s} : nonSPVReg s -> vreg s  := 
+  match s return nonSPVReg s -> vreg s with 
+    | OpSize1 => fun r =>
+                   match r with
+                     | mkNonSPReg8 r => mkGPReg8 (mkGPReg r)
+                   end
+    | OpSize2 => fun r =>
+                   match r with
+                     | mkNonSPReg16 r => mkReg16 (mkGPReg r)
+                   end
+    | OpSize4 => fun r =>
+                   match r with
+                     | mkNonSPReg32 r => mkReg32 (mkGPReg r)
+                   end
+    | OpSize8 => fun r => r
+  end. 
+
+Coercion gpVReg_to_vreg {s} : gpVReg s -> vreg s  := 
+  match s return gpVReg s -> vreg s with 
+    | OpSize1 => fun r => r
+    | OpSize2 => fun r =>
+                   match r with
+                     | mkGPReg16 r => mkReg16 r
+                   end
+    | OpSize4 => fun r =>
+                   match r with
+                     | mkGPReg32 r => mkReg32 r
+                   end
+    | OpSize8 => fun r => r
+  end. 
+
+
 
 Inductive SSEreg := YMM0 | YMM1 | YMM2  | YMM3  | YMM4  | YMM5  | YMM6 | YMM7
                   | YMM8 | YMM9 | YMM10 | YMM11 | YMM12 | YMM13 | YMM14 | YMM15.
@@ -165,8 +284,18 @@ Notation XMM7 := (mkXMMreg YMM7).
 Notation XMM8 := (mkXMMreg YMM8).
 Notation XMM9 := (mkXMMreg YMM9).
 Notation XMM10 := (mkXMMreg YMM10).
-Notation XMM11 := (mkXMMreg YMM1).
+Notation XMM11 := (mkXMMreg YMM11).
 Notation XMM12 := (mkXMMreg YMM12).
 Notation XMM13 := (mkXMMreg YMM13).
 Notation XMM14 := (mkXMMreg YMM14).
 Notation XMM15 := (mkXMMreg YMM15).
+
+Definition XMMreg_toNat r :=
+  (* TODO: don't think is correct wrt. the encoding *)
+  match r with XMM0 => 0 | XMM1 => 1 | XMM2 => 2 | XMM3 => 3 | XMM4 => 4
+            | XMM5 => 5 | XMM6 => 6 | XMM7 => 7 
+            | XMM8 => 8 | XMM9 => 9 | XMM10 => 10 | XMM11 => 11
+            | XMM12 => 12 | XMM13 => 13 | XMM14 => 14 | XMM15 => 15 end.
+Lemma XMMreg_toNat_inj : injective XMMreg_toNat. Proof. by repeat case => //. Qed.
+Canonical Structure XMMreg_EqMixin := InjEqMixin XMMreg_toNat_inj.
+Canonical Structure XMMreg_EqType := Eval hnf in EqType _ XMMreg_EqMixin.
